src/Implementations/File/File.v
@@ -1,5 +1,5 @@
 Require Import Framework FSParameters AuthenticatedDiskLayer BlockAllocator Inode.
-Require Import FunctionalExtensionality Lia.
+Require Import Compare_dec FunctionalExtensionality Lia.
 Import IfNotations.
 
 Module DiskAllocatorParams <: BlockAllocatorParameters.
@@ -17,7 +17,9 @@ Definition file_rep (file: File) (inode: Inode) (file_block_map: disk value) :=
   length file.(blocks) = length inode.(block_numbers) /\
   (forall i block_number,
        nth_error inode.(block_numbers) i = Some block_number ->
-       nth_error file.(blocks) i = file_block_map block_number).
+       exists block,
+         nth_error file.(blocks) i = Some block /\
+         file_block_map block_number = Some block).
 
 Definition file_map_rep (file_disk: @mem Inum addr_dec File) inode_map file_block_map :=
    addrs_match_exactly file_disk inode_map /\
@@ -199,7 +201,8 @@ Proof.
         apply Some_injective.
         repeat rewrite <- nth_error_nth'; try lia.
         destruct_fresh (nth_error (block_numbers i) pos).
-        erewrite H7, H10; eauto.
+        eapply_fresh H7 in D2; eauto; cleanup.
+        eapply_fresh H10 in D2; eauto; cleanup; eauto.
         apply nth_error_None in D2; lia.
       }
       rewrite A; eauto.
@@ -249,6 +252,55 @@ Proof.
 Qed.
 
 (*** Specs ***)
+(*
+Lemma auth_then_exec_finished:
+    forall u T (p: Inum -> prog _ (option T)) o s s' r inum fd (pred_s_r: _ -> _ -> _ -> Prop),
+    files_rep fd s ->
+    (forall sx o_p fdp sp rp,
+       files_inner_rep fdp (fst sx) ->
+       exec (TransactionalDiskLang data_length) u o_p sx (p inum) (Finished sp rp) ->
+       pred_s_r sx sp rp) ->  
+    exec AuthenticatedDiskLang u o s (auth_then_exec inum p) (Finished s' r) ->
+    files_rep fd s' /\
+    ((r = None /\
+      (inum >= inode_count \/
+       fd inum = None \/
+       (exists file,
+          fd inum = Some file /\
+          file.(BaseTypes.owner) <> u))
+      /\ files_rep fd s') \/
+     (exists f v,
+        r = Some v /\
+        fd inum = Some f /\
+        inum < inode_count /\
+        f.(BaseTypes.owner) = u /\
+        pred_s_r (snd s) (snd s') r)).
+Proof.
+  unfold auth_then_exec; intros; simpl.
+  repeat invert_exec.
+  simpl in *; repeat cleanup_pairs.
+  
+  unfold files_rep, files_inner_rep in H; simpl in *; cleanup. 
+  eapply get_owner_finished in H4; eauto.
+  2: rewrite H; eauto.
+
+  cleanup; split_ors; cleanup.
+  {
+    repeat cleanup_pairs.
+    eapply H0 in H8.
+    2: {
+      unfold files_inner_rep.
+      eexists; intuition eauto.
+      simpl.
+      eexists; intuition eauto.
+      
+    
+    Search lift_L2.
+    econstructor; eauto.
+    intuition eauto.
+    eexists; intuition eauto.
+ *)
+  
 Lemma read_finished:
   forall u o s s' r inum off fd,
     files_rep fd s ->
@@ -265,8 +317,287 @@ Lemma read_finished:
         fd inum = Some f /\
         inum < inode_count /\
         f.(BaseTypes.owner) = u)).
-Admitted.
+Proof.
+  unfold read, auth_then_exec, read_inner;
+  intros; simpl.
+  repeat invert_exec;
+  simpl in *; repeat cleanup_pairs; eauto.
+  { (** Success **)
+    unfold files_rep, files_inner_rep in H; simpl in *; cleanup.
+    repeat cleanup_pairs.
+    eapply get_owner_finished in H3; eauto.
+    simpl in *; cleanup; split_ors; cleanup.
+    eapply get_block_number_finished in H7; eauto.
+    simpl in *; cleanup; split_ors; cleanup.
+    repeat cleanup_pairs.
+    eapply DiskAllocator.block_allocator_rep_inbounds_eq with (s2:= t1) in H1.    
+    eapply DiskAllocator.read_finished in H8; eauto.
+    simpl in *.
+    cleanup; split_ors; cleanup.
+    unfold inode_rep in *; cleanup.
+    eapply InodeAllocator.block_allocator_rep_inbounds_eq with (s2:= t) in H6.
+    clear H0 H1 H3 H4 H7 H10.
+    repeat (split; eauto).
+    {
+      unfold files_inner_rep, inode_rep; simpl.
+      eexists; intuition eauto.
+    }
+    {
+      destruct_fresh (fd inum).
+      {
+        unfold file_map_rep in *; cleanup.
+        eapply_fresh H1 in H5; eauto.
+        unfold file_rep in *; cleanup; eauto.
+                
+        right; eexists; intuition eauto.
+        edestruct H4; eauto; cleanup.
+        apply nth_error_nth'; eauto.
+        rewrite nth_selN_eq in H11;
+        erewrite H10 in H11; cleanup; eauto.
+        {
+          unfold block_allocator_rep,
+          inode_map_rep in *; cleanup.
+          rewrite H7 in H5; simpl in *.
+          unfold InodeAllocatorParams.num_of_blocks in *.
+          destruct (lt_dec inum inode_count); eauto.
+          rewrite H15 in H5; simpl in *; try congruence; try lia.
+        }
+      }
+      {
+        unfold file_map_rep, addrs_match_exactly in *; cleanup.
+        edestruct H0; exfalso.
+        eapply H3; eauto; congruence.
+      }
+    }
+    {
+      intros.
+      pose proof inodes_before_data.
+      apply H10;
+      unfold DiskAllocatorParams.bitmap_addr,
+      DiskAllocatorParams.num_of_blocks,
+      InodeAllocatorParams.bitmap_addr,
+      InodeAllocatorParams.num_of_blocks in *;
+      try lia.
+    }
+    {
+      intros.
+      pose proof inodes_before_data.
+      rewrite H7. apply H4.
+      all:
+        unfold DiskAllocatorParams.bitmap_addr,
+        DiskAllocatorParams.num_of_blocks,
+        InodeAllocatorParams.bitmap_addr,
+        InodeAllocatorParams.num_of_blocks in *;
+      try lia.
+    }
+  }
+  { (** Read Failed **)
+    unfold files_rep, files_inner_rep in H; simpl in *; cleanup.
+    repeat cleanup_pairs.
+    eapply get_owner_finished in H3; eauto.
+    simpl in *; cleanup; split_ors; cleanup.
+    eapply get_block_number_finished in H7; eauto.
+    simpl in *; cleanup; split_ors; cleanup.
+    repeat cleanup_pairs.
+    eapply_fresh (DiskAllocator.block_allocator_rep_inbounds_eq x1 t1 t) in H1.    
+    eapply DiskAllocator.read_finished in H8; eauto.
+    simpl in *.
+    cleanup; split_ors; cleanup.
+    unfold inode_rep in *; cleanup.
+    eapply (InodeAllocator.block_allocator_rep_inbounds_eq x2 t (fst s0)) in H6.
+    repeat (split; eauto).
+    {
+      unfold files_inner_rep, inode_rep; simpl.
+      eexists; intuition eauto.
+    }
+    {
+      left.
+      unfold inode_map_rep, inode_map_valid in *; cleanup.
+      eapply_fresh H18 in H5; unfold inode_valid in *.
+      cleanup.
+      eapply Forall_forall in H15; [| apply in_selN; eauto].
+      unfold file_map_rep in *; cleanup.
+      destruct_fresh (fd inum).
+      eapply_fresh f in H5; eauto.
+      unfold file_rep in *; cleanup.
+      unfold DiskAllocator.block_allocator_rep in *; cleanup.
+      eapply_fresh (DiskAllocator.valid_bits_extract x1 x7
+       (bits (value_to_bits (fst s0 DiskAllocatorParams.bitmap_addr)))
+       (selN (block_numbers x) off 0)) in v; eauto.
+      cleanup; try congruence.
 
+      split_ors; cleanup.
+      edestruct H17; eauto; cleanup.
+      apply nth_error_nth'; eauto.
+      rewrite nth_selN_eq in H11; cleanup.
+      rewrite H21 in H11; cleanup.
+
+      {
+        edestruct H17; eauto; cleanup.
+        apply nth_error_nth'; eauto.
+        destruct (lt_dec (selN (block_numbers x) off 0) DiskAllocatorParams.num_of_blocks); eauto.
+        rewrite e7 in H9; cleanup.
+        instantiate (1:= 0);
+        rewrite <- nth_selN_eq; lia.
+      }
+      rewrite bitlist_length.      
+      pose proof DiskAllocatorParams.num_of_blocks_in_bounds.
+      unfold DiskAllocatorParams.num_of_blocks in *;
+      lia.
+
+      - edestruct a.
+        exfalso; apply H16; eauto; congruence.
+    }
+    {
+      intros.
+      pose proof inodes_before_data.
+      apply H10;
+      unfold DiskAllocatorParams.bitmap_addr,
+      DiskAllocatorParams.num_of_blocks,
+      InodeAllocatorParams.bitmap_addr,
+      InodeAllocatorParams.num_of_blocks in *;
+      try lia.
+    }
+    {
+      intros.
+      pose proof inodes_before_data.
+      rewrite H7. apply H4.
+      all:
+        unfold DiskAllocatorParams.bitmap_addr,
+        DiskAllocatorParams.num_of_blocks,
+        InodeAllocatorParams.bitmap_addr,
+        InodeAllocatorParams.num_of_blocks in *;
+      try lia.
+    }
+  }
+  { (** off is out-of-bounds **)
+    unfold files_rep, files_inner_rep in H; simpl in *; cleanup.
+    repeat cleanup_pairs.
+    eapply get_owner_finished in H3; eauto.
+    simpl in *; cleanup; split_ors; cleanup.
+    eapply get_block_number_finished in H7; eauto.
+    simpl in *; cleanup; split_ors; cleanup.
+    repeat cleanup_pairs.
+    eapply_fresh (DiskAllocator.block_allocator_rep_inbounds_eq x1 t1 t) in H1.  
+    repeat (split; eauto).
+    {
+      unfold files_inner_rep, inode_rep; simpl.
+      eexists; intuition eauto.
+    }
+    {
+      split_ors; cleanup.
+      destruct_fresh (fd inum).
+      {
+        unfold file_map_rep in *; cleanup.
+        eapply_fresh H2 in H5; eauto.
+        unfold file_rep in *; cleanup; eauto.
+        
+        right; eexists; intuition eauto.        
+        symmetry; apply nth_error_None; lia.
+        
+        {
+          unfold inode_rep, block_allocator_rep,
+          inode_map_rep in *; cleanup.
+          rewrite H12 in H5; simpl in *.
+          unfold InodeAllocatorParams.num_of_blocks in *.
+          destruct (lt_dec inum inode_count); eauto.
+          rewrite H16 in H5; simpl in *; try congruence; try lia.
+        }
+      }
+      {
+        unfold file_map_rep, addrs_match_exactly in *; cleanup.
+        edestruct H; exfalso.
+        eapply H10; eauto; congruence.
+      }
+    }
+    {
+      intros.
+      pose proof inodes_before_data.
+      rewrite H7. apply H4.
+      all:
+        unfold DiskAllocatorParams.bitmap_addr,
+        DiskAllocatorParams.num_of_blocks,
+        InodeAllocatorParams.bitmap_addr,
+        InodeAllocatorParams.num_of_blocks in *;
+      try lia.
+    }
+  }
+  { (** Auth failed **) 
+    unfold files_rep, files_inner_rep in H; simpl in *; cleanup.
+    repeat cleanup_pairs.
+    eapply get_owner_finished in H3; eauto.
+    simpl in *; cleanup; split_ors; cleanup.
+    eapply_fresh (DiskAllocator.block_allocator_rep_inbounds_eq x0 (snd s0) (fst s0)) in H1.  
+    repeat (split; eauto).
+    {
+      unfold files_inner_rep, inode_rep; simpl.
+      eexists; intuition eauto.
+    }
+    {
+      destruct_fresh (fd inum).
+      {
+        unfold file_map_rep in *; cleanup.
+        eapply_fresh H2 in H5; eauto.
+        unfold file_rep in *; cleanup; eauto.
+        
+        left; intuition eauto.
+        right; right; eexists; intuition eauto.
+        congruence.
+      }
+      {
+        unfold file_map_rep, addrs_match_exactly in *; cleanup.
+        edestruct H; exfalso.
+        eapply H7; eauto; congruence.
+      }
+    }
+    {
+      intros.
+      pose proof inodes_before_data.
+      apply H4.
+      all:
+        unfold DiskAllocatorParams.bitmap_addr,
+        DiskAllocatorParams.num_of_blocks,
+        InodeAllocatorParams.bitmap_addr,
+        InodeAllocatorParams.num_of_blocks in *;
+      try lia.
+    }
+  }
+  { (** inum doesn't exists **)
+    unfold files_rep, files_inner_rep in H; simpl in *; cleanup.
+    repeat cleanup_pairs.
+    eapply get_owner_finished in H3; eauto.
+    simpl in *; cleanup; split_ors; cleanup.
+    eapply_fresh (DiskAllocator.block_allocator_rep_inbounds_eq x0 (snd s1) (fst s1)) in H1.  
+    repeat (split; eauto).
+    {
+      unfold files_inner_rep, inode_rep; simpl.
+      eexists; intuition eauto.
+    }
+    left; intuition eauto.
+    destruct_fresh (fd inum).
+    {
+      unfold file_map_rep, addrs_match_exactly in *; cleanup.
+      edestruct H; exfalso.
+      eapply H6; eauto; congruence.
+    }
+    intuition.
+    {
+      intros.
+      pose proof inodes_before_data.
+      apply H4.
+      all:
+        unfold DiskAllocatorParams.bitmap_addr,
+        DiskAllocatorParams.num_of_blocks,
+        InodeAllocatorParams.bitmap_addr,
+        InodeAllocatorParams.num_of_blocks in *;
+      try lia.
+    }
+  }
+  Unshelve.
+  eauto.
+Qed.    
+     
+  
 Lemma read_crashed:
   forall u o s s' inum off fm,
     files_rep fm s ->
