src/Implementations/Inode/Inode.v
@@ -1,5 +1,5 @@
 Require Import Framework FSParameters TransactionalDiskLayer BlockAllocator.
-Require Import FunctionalExtensionality.
+Require Import FunctionalExtensionality Lia.
 Import IfNotations.
 
 (*** Definitions ***)
@@ -122,6 +122,16 @@ Proof.
   rewrite H2, H; eauto.
 Qed.
 
+Lemma nth_error_some_lt:
+  forall T (l: list T) n t,
+    nth_error l n = Some t ->
+    n < length l.
+Proof.
+  induction l; simpl; intros; eauto;
+  destruct n; simpl in *; cleanup.
+  lia.
+  apply IHl in H; lia.
+Qed.
 
 (*** Specs ***)
 Theorem alloc_finished:
@@ -131,7 +141,10 @@ Theorem alloc_finished:
     ((exists a, t = Some a /\
           dh a = None /\
           inode_rep (Mem.upd dh a (Build_Inode user [])) (fst s')) \/
-    (t = None /\ inode_rep dh (fst s'))) /\
+     (t = None /\ inode_rep dh (fst s'))) /\
+    (forall a, a < InodeAllocatorParams.bitmap_addr \/
+          a > InodeAllocatorParams.bitmap_addr + InodeAllocatorParams.num_of_blocks ->
+          fst s' a = fst s a) /\
      snd s' = snd s.
 Proof.
   unfold alloc, inode_rep; intros; cleanup.
@@ -142,7 +155,7 @@ Proof.
     left; eexists; intuition eauto.
     {
       unfold inode_map_rep in *; cleanup.
-      rewrite H0, H3; simpl; eauto.
+      rewrite H0, H4; simpl; eauto.
     }
     {
       eexists; intuition eauto.
@@ -160,30 +173,30 @@ Proof.
         split; intros.
         {
           destruct (addr_dec x0 i); subst.
-          - rewrite Mem.upd_eq in H6; simpl; eauto.
+          - rewrite Mem.upd_eq in H7; simpl; eauto.
             cleanup.
             unfold inode_valid; simpl; eauto.
             split; constructor.
-          - rewrite Mem.upd_ne in H6; simpl; eauto.
+          - rewrite Mem.upd_ne in H7; simpl; eauto.
         }
         {
           destruct (addr_dec x0 i); subst.
-          - rewrite Mem.upd_eq in H7; simpl; eauto.
+          - rewrite Mem.upd_eq in H8; simpl; eauto.
             cleanup; simpl.
-            rewrite Mem.upd_ne in H8; simpl; eauto.
-            apply H1 in H8.
+            rewrite Mem.upd_ne in H9; simpl; eauto.
+            apply H1 in H9.
             unfold inode_valid in *;
             cleanup; eauto.
             
-          - rewrite Mem.upd_ne in H7; simpl; eauto.
+          - rewrite Mem.upd_ne in H8; simpl; eauto.
             destruct (addr_dec x0 j); subst.
-            rewrite Mem.upd_eq in H8; simpl; eauto.
+            rewrite Mem.upd_eq in H9; simpl; eauto.
             cleanup; simpl.
             rewrite app_nil_r.
-            apply H1 in H7.
+            apply H1 in H8.
             unfold inode_valid in *;
             cleanup; eauto.
-            rewrite Mem.upd_ne in H8; simpl; eauto.
+            rewrite Mem.upd_ne in H9; simpl; eauto.
         }
       }
     }
@@ -196,7 +209,10 @@ Theorem free_finished:
     exec (TransactionalDiskLang data_length) u o s (free inum) (Finished s' t) ->
     ((t = Some tt /\
       (inode_rep dh (fst s') \/ inode_rep (Mem.delete dh inum) (fst s'))) \/
-    (t = None /\ inode_rep dh (fst s'))) /\
+     (t = None /\ inode_rep dh (fst s'))) /\
+    (forall a, a < InodeAllocatorParams.bitmap_addr \/
+          a > InodeAllocatorParams.bitmap_addr + InodeAllocatorParams.num_of_blocks ->
+          fst s' a = fst s a) /\
      snd s' = snd s.
 Proof.
   unfold free, inode_rep; intros; cleanup.
@@ -224,17 +240,17 @@ Proof.
            split; intros.
            {
              destruct (addr_dec inum i); subst.
-             - rewrite Mem.delete_eq in H5; simpl; eauto; congruence.
-             - rewrite Mem.delete_ne in H5; simpl; eauto.
+             - rewrite Mem.delete_eq in H6; simpl; eauto; congruence.
+             - rewrite Mem.delete_ne in H6; simpl; eauto.
            }
            {
              destruct (addr_dec inum i); subst.
-             - rewrite Mem.delete_eq in H6; simpl; eauto; congruence.
+             - rewrite Mem.delete_eq in H7; simpl; eauto; congruence.
                
-             - rewrite Mem.delete_ne in H6; simpl; eauto.
+             - rewrite Mem.delete_ne in H7; simpl; eauto.
                destruct (addr_dec inum j); subst.
-               rewrite Mem.delete_eq in H7; simpl; eauto; congruence.
-               rewrite Mem.delete_ne in H7; simpl; eauto.
+               rewrite Mem.delete_eq in H8; simpl; eauto; congruence.
+               rewrite Mem.delete_ne in H8; simpl; eauto.
            }
          }
       }
@@ -248,8 +264,12 @@ Theorem get_inode_finished:
   forall dh u o s inum t s',
     inode_rep dh (fst s) ->
     exec (TransactionalDiskLang data_length) u o s (get_inode inum) (Finished s' t) ->
-    ((exists inode, t = Some inode /\ dh inum = Some inode) \/ t = None) /\
+    ((exists inode, t = Some inode /\ dh inum = Some inode) \/
+     (t = None /\ dh inum = None)) /\
     inode_rep dh (fst s') /\
+    (forall a, a < InodeAllocatorParams.bitmap_addr \/
+          a > InodeAllocatorParams.bitmap_addr + InodeAllocatorParams.num_of_blocks ->
+          fst s' a = fst s a) /\
     snd s' = snd s.
 Proof.
   unfold get_inode, inode_rep; intros; cleanup.
@@ -261,6 +281,11 @@ Proof.
     unfold inode_map_rep in *; cleanup.
     left; rewrite H0; cleanup; simpl; eauto.
   }
+  {
+    unfold inode_map_rep in *; cleanup.
+    right; split; eauto.
+    rewrite H0, H5; simpl; eauto.
+  }    
 Qed.
 
 
@@ -276,6 +301,9 @@ Theorem set_inode_finished:
     ((t = Some tt /\
       (inode_rep dh (fst s') \/ inode_rep (Mem.upd dh inum inode) (fst s'))) \/
      (t = None /\ inode_rep dh (fst s'))) /\
+    (forall a, a < InodeAllocatorParams.bitmap_addr \/
+          a > InodeAllocatorParams.bitmap_addr + InodeAllocatorParams.num_of_blocks ->
+          fst s' a = fst s a) /\
     snd s' = snd s.
 Proof.
   unfold set_inode, inode_rep; intros; cleanup.
@@ -300,23 +328,23 @@ Proof.
         split; intros.
         {
           destruct (addr_dec inum i); subst.
-          - rewrite Mem.upd_eq in H7; simpl; eauto.
+          - rewrite Mem.upd_eq in H8; simpl; eauto.
             cleanup.
             unfold inode_valid; simpl; eauto.
-          - rewrite Mem.upd_ne in H7; simpl; eauto.
+          - rewrite Mem.upd_ne in H8; simpl; eauto.
         }
         {
           destruct (addr_dec inum i); subst.
-          - rewrite Mem.upd_eq in H8; simpl; eauto.
+          - rewrite Mem.upd_eq in H9; simpl; eauto.
             cleanup; simpl.
-            rewrite Mem.upd_ne in H9; simpl; eauto.
+            rewrite Mem.upd_ne in H10; simpl; eauto.
             
-          - rewrite Mem.upd_ne in H8; simpl; eauto.
+          - rewrite Mem.upd_ne in H9; simpl; eauto.
             destruct (addr_dec inum j); subst.
-            rewrite Mem.upd_eq in H9; simpl; eauto.
+            rewrite Mem.upd_eq in H10; simpl; eauto.
             cleanup; simpl.
             apply NoDup_app_comm; eauto.
-            rewrite Mem.upd_ne in H9; simpl; eauto.
+            rewrite Mem.upd_ne in H10; simpl; eauto.
         }
       }
   }
@@ -336,6 +364,9 @@ Theorem extend_finished:
         (inode_rep dh (fst s') \/
          inode_rep (Mem.upd dh inum (Build_Inode inode.(owner) (inode.(block_numbers) ++ [block_num]))) (fst s'))) \/
      (t = None /\ inode_rep dh (fst s'))) /\
+    (forall a, a < InodeAllocatorParams.bitmap_addr \/
+          a > InodeAllocatorParams.bitmap_addr + InodeAllocatorParams.num_of_blocks ->
+          fst s' a = fst s a) /\
     snd s' = snd s.
 Proof.
   unfold extend; intros; cleanup.
@@ -345,12 +376,20 @@ Proof.
   split_ors; cleanup;
   eapply set_inode_finished in H3; simpl; eauto; cleanup.
   split_ors; cleanup;
-  split; eauto.
+  repeat (split; eauto).
+  {
+    intros.
+    rewrite H3; eauto.    
+  }
+  {
+    intros.
+    rewrite H3; eauto.    
+  }
   {
     unfold inode_valid; simpl.
     unfold inode_rep, inode_map_rep,
     inode_map_valid in *; cleanup.
-    eapply_fresh H10 in H6;
+    eapply_fresh H11 in H7;
     unfold inode_valid in Hx; cleanup; eauto.    
     split; eauto.
     - apply NoDup_app_comm; simpl.
@@ -383,6 +422,9 @@ Theorem change_owner_finished:
         (inode_rep dh (fst s') \/
          inode_rep (Mem.upd dh inum (Build_Inode new_owner inode.(block_numbers))) (fst s'))) \/
      (t = None /\ inode_rep dh (fst s'))) /\
+    (forall a, a < InodeAllocatorParams.bitmap_addr \/
+          a > InodeAllocatorParams.bitmap_addr + InodeAllocatorParams.num_of_blocks ->
+          fst s' a = fst s a) /\
     snd s' = snd s.
 Proof.
   unfold change_owner; intros; cleanup.
@@ -392,12 +434,14 @@ Proof.
   split_ors; cleanup;
   eapply set_inode_finished in H1; simpl; eauto; cleanup.
   split_ors; cleanup;
-  split; eauto.
+  repeat (split; eauto).
+  { intros; rewrite H1; eauto. }
+  { intros; rewrite H1; eauto. }
   {
     unfold inode_valid; simpl.
     unfold inode_rep, inode_map_rep,
     inode_map_valid in *; cleanup.
-    eapply_fresh H8 in H4;
+    eapply_fresh H9 in H5;
     unfold inode_valid in Hx; cleanup; eauto.
   }
   {
@@ -411,20 +455,37 @@ Theorem get_block_number_finished:
   forall dh u o s inum off t s',
     inode_rep dh (fst s) ->
     exec (TransactionalDiskLang data_length) u o s (get_block_number inum off) (Finished s' t) ->
-    ((exists inode, t = Some (selN (inode.(block_numbers)) off 0) /\ dh inum = Some inode) \/ t = None) /\
+    ((exists inode, off < length (inode.(block_numbers)) /\
+               t = Some (selN (inode.(block_numbers)) off 0) /\ dh inum = Some inode) \/
+     (t = None /\ (dh inum = None \/
+                  (exists inode, dh inum = Some inode /\ off >= length (inode.(block_numbers)))))) /\
     inode_rep dh (fst s') /\
+    (forall a, a < InodeAllocatorParams.bitmap_addr \/
+          a > InodeAllocatorParams.bitmap_addr + InodeAllocatorParams.num_of_blocks ->
+          fst s' a = fst s a) /\
     snd s' = snd s.
 Proof.
   unfold get_block_number; intros; cleanup.
   repeat invert_exec;
   eapply get_inode_finished in H0; eauto;
   cleanup; eauto;
-  split; eauto.
-  destruct_fresh (nth_error (block_numbers i) off); eauto.
+  split; eauto;
   split_ors; cleanup.
-  left; eexists; split; eauto.
-  rewrite nth_selN_eq.
-  erewrite nth_error_nth; eauto.
+  {    
+    destruct_fresh (nth_error (block_numbers x0) off); eauto.  
+    {
+      left; eexists; split; eauto.
+      eapply nth_error_some_lt; eauto.
+      rewrite nth_selN_eq.
+      erewrite nth_error_nth; eauto.
+    }
+    {
+      right; intuition eauto.
+      right; eexists; split; eauto.
+      apply nth_error_None; eauto.
+    }
+  }
+  right; intuition eauto.  
 Qed.
 
 Theorem get_all_block_numbers_finished:
@@ -433,6 +494,9 @@ Theorem get_all_block_numbers_finished:
     exec (TransactionalDiskLang data_length) u o s (get_all_block_numbers inum) (Finished s' t) ->
     ((exists inode, t = Some (inode.(block_numbers)) /\ dh inum = Some inode) \/ t = None) /\
     inode_rep dh (fst s') /\
+    (forall a, a < InodeAllocatorParams.bitmap_addr \/
+          a > InodeAllocatorParams.bitmap_addr + InodeAllocatorParams.num_of_blocks ->
+          fst s' a = fst s a) /\
     snd s' = snd s.
 Proof.
   unfold get_all_block_numbers; intros; cleanup.
@@ -447,8 +511,12 @@ Theorem get_owner_finished:
   forall dh u o s inum t s',
     inode_rep dh (fst s) ->
     exec (TransactionalDiskLang data_length) u o s (get_owner inum) (Finished s' t) ->
-    ((exists inode, t = Some inode.(owner) /\ dh inum = Some inode) \/ t = None) /\
+    ((exists inode, t = Some inode.(owner) /\ dh inum = Some inode) \/
+     (t = None /\ dh inum = None)) /\
     inode_rep dh (fst s') /\
+    (forall a, a < InodeAllocatorParams.bitmap_addr \/
+          a > InodeAllocatorParams.bitmap_addr + InodeAllocatorParams.num_of_blocks ->
+          fst s' a = fst s a) /\
     snd s' = snd s.
 Proof.
   unfold get_owner; intros; cleanup.
@@ -457,497 +525,8 @@ Proof.
   cleanup; eauto;
   split; eauto.
   split_ors; cleanup; eauto.
+  split_ors; cleanup; intuition eauto.
 Qed.
 
-(*
-Theorem get_inode_ok:
-  forall inum s' t imap F,
-    strongest_postcondition (TransactionalDiskLang data_length) (get_inode inum)
-                            (fun o s => (F * inode_rep imap)%predicate (mem_union (fst s) (snd s))) t s' ->
-    (t = imap inum /\ (F * inode_rep imap)%predicate (mem_union (fst s') (snd s'))).
-Proof.
-  unfold inode_rep; intros; simpl in *; cleanup.
-  destruct x; simpl in *; cleanup.
-  -    
-    eapply sp_impl in H.
-    eapply (sp_exists_extract (disk value)) with (P:=fun inode_block_map o s =>  (F *
-   (block_allocator_rep inode_block_map *
-    [[forall i : addr, imap i = option_map decode_inode (inode_block_map i)]] *
-    [[forall (i : addr) (inode : Inode),
-      imap i = Some inode -> compatible_inode imap i inode]]))%predicate
-    (mem_union (fst s) (snd s))) in H.
-    cleanup.
-    eapply sp_impl in H.
-    apply read_ok in H.
-    2: {
-      intros; cleanup.
-      simpl; eauto.
-      instantiate (1:= x).
-      instantiate (1:= F * [[forall i : addr, imap i = option_map decode_inode (x i)]] * [[forall (i : addr) (inode : Inode),
-      imap i = Some inode -> compatible_inode imap i inode]]).
-      pred_apply' H0; cancel.
-    }
-    
-    cleanup.
-    destruct_lift H0.
-    rewrite H5; cleanup.
-    rewrite <- H; simpl.
-    intuition eauto.
-    pred_apply; cancel.
-    exists x; pred_apply; cancel.
-
-    simpl; intros; cleanup.
-    apply pimpl_exists_l_star_r in H0.
-    destruct H0.
-    exists x; eauto.
-    
-  -
-    eapply sp_impl in H.
-    eapply (sp_exists_extract (disk value)) with (P:=fun inode_block_map o s =>  (F *
-   (block_allocator_rep inode_block_map *
-    [[forall i : addr, imap i = option_map decode_inode (inode_block_map i)]] *  [[forall (i : addr) (inode : Inode),
-      imap i = Some inode -> compatible_inode imap i inode]]))%predicate
-    (mem_union (fst s) (snd s))) in H.
-    cleanup.
-    eapply sp_impl in H.
-    apply read_ok in H.
-    2: {
-      intros; cleanup.
-      simpl; eauto.
-      instantiate (1:= x).
-      instantiate (1:= F * [[forall i : addr, imap i = option_map decode_inode (x i)]] * [[forall (i : addr) (inode : Inode),
-      imap i = Some inode -> compatible_inode imap i inode]]).
-      pred_apply' H0; cancel.
-    }
-    
-    cleanup.
-    destruct_lift H0.
-    rewrite H5; cleanup.
-    rewrite <- H; simpl.
-    intuition eauto.
-    pred_apply; cancel.
-    exists x; pred_apply; cancel.
-
-    simpl; intros; cleanup.
-    apply pimpl_exists_l_star_r in H0.
-    destruct H0.
-    exists x; eauto.
-Qed.
-
-
-Theorem set_inode_ok:
-  forall inum inode s' t imap F,
-    strongest_postcondition (TransactionalDiskLang data_length) (set_inode inum inode)
-                            (fun o s => (F * inode_rep imap)%predicate (mem_union (fst s) (snd s)) /\
-                                     compatible_inode imap inum inode /\
-                            (forall tok, In tok o -> tok <> OpOracle (TransactionalDiskOperation data_length) [TxnFull])%list ) t s' ->
-    (exists i, imap inum = Some i /\ t = Some tt /\ (F * inode_rep (upd imap inum inode))%predicate (mem_union (fst s') (snd s'))) \/
-    (t = None /\ (F * inode_rep imap)%predicate (mem_union (fst s') (snd s'))).
-Proof.
-  unfold inode_rep; intros; simpl in *; cleanup.
-  eapply sp_impl in H.
-  eapply (sp_exists_extract (disk value)) with (P:=fun inode_block_map o s =>  (F *
-   (block_allocator_rep inode_block_map *
-    [[forall i : addr, imap i = option_map decode_inode (inode_block_map i)]] * [[forall (i : addr) (inode : Inode),
-      imap i = Some inode -> compatible_inode imap i inode]]))%predicate
-                                                             (mem_union (fst s) (snd s)) /\
-                                                                            compatible_inode imap inum inode /\
-                                               (forall tok, In tok o -> tok <> OpOracle (TransactionalDiskOperation data_length) [TxnFull])%list) in H.
-    cleanup.
-    eapply sp_impl in H.
-    apply write_ok in H.
-    2: {
-      intros; cleanup.
-      simpl; eauto.
-      instantiate (1:= x0).
-      instantiate (1:= F * [[forall i : addr, imap i = option_map decode_inode (x0 i)]] *
-     [[forall (i : addr) (inode : Inode),
-      imap i = Some inode -> compatible_inode imap i inode]] * [[compatible_inode imap inum inode ]]).
-      split; eauto.
-      pred_apply' H0; cancel.
-    }
-    split_ors; cleanup.
-    
-  -    destruct_lift H1.
-    left; eexists; intuition eauto.
-    rewrite H6, H; simpl; eauto.
-    pred_apply; cancel.
-    exists (upd x0 inum (encode_inode inode)).
-    pred_apply; cancel.
-    destruct (addr_dec inum i); subst;
-    [ repeat rewrite upd_eq | repeat rewrite upd_ne]; simpl; eauto.
-    rewrite inode_encode_decode; eauto.
-
-    unfold compatible_inode in *;
-    destruct (addr_eq_dec inum i); subst;
-    [ repeat rewrite upd_eq | repeat rewrite upd_ne]; simpl; eauto.
-    rewrite upd_eq in H2; eauto; cleanup.
-    intuition.
-    rewrite upd_ne in H7; eauto.
-
-    rewrite upd_ne in H2; eauto; cleanup.
-    specialize H5 with (1:= H2); cleanup.
-    intuition.
-     destruct (addr_eq_dec inum j); subst;
-    [ repeat rewrite upd_eq | repeat rewrite upd_ne]; simpl; eauto.
-     rewrite upd_eq in H9; eauto; cleanup.
-     apply NoDup_app_comm;
-     eapply H4; eauto.
-     rewrite upd_ne in H9; eauto.
-    
-  - right; intuition cleanup.
-    pred_apply; cancel.
-    exists x0.
-    pred_apply; cancel.
-    
- - simpl; intros; cleanup.
-   apply pimpl_exists_l_star_r in H0.
-   destruct H0.
-   exists x0; intuition eauto.
-Qed.
-
-Global Opaque get_inode set_inode.
-
-Theorem alloc_ok:
-  forall user s' t imap F,
-    strongest_postcondition (TransactionalDiskLang data_length) (alloc user)
-                            (fun o s => (F * inode_rep imap)%predicate (mem_union (fst s) (snd s)) /\
-                            (forall tok, In tok o -> tok <> OpOracle (TransactionalDiskOperation data_length) [TxnFull])%list ) t s' ->
-    (exists inum, t = Some inum /\ imap inum = None /\ (F * inode_rep (upd imap inum (Build_Inode user [])))%predicate (mem_union (fst s') (snd s'))) \/
-    (t = None /\ (F * inode_rep imap)%predicate (mem_union (fst s') (snd s'))).
-Proof.
-    unfold inode_rep; intros; simpl in *; cleanup.
-  eapply sp_impl in H.
-  eapply (sp_exists_extract (disk value)) with (P:=fun inode_block_map o s =>  (F *
-   (block_allocator_rep inode_block_map *
-    [[forall i : addr, imap i = option_map decode_inode (inode_block_map i)]] *
-    [[forall (i : addr) (inode : Inode),
-      imap i = Some inode -> compatible_inode imap i inode]]))%predicate
-                                                                          (mem_union (fst s) (snd s)) /\
-                                               (forall tok, In tok o -> tok <> OpOracle (TransactionalDiskOperation data_length) [TxnFull])%list) in H.
-    cleanup.
-    eapply sp_impl in H.
-    apply alloc_ok in H.
-    2: {
-      intros; cleanup.
-      simpl; eauto.
-      instantiate (1:= x0).
-      instantiate (1:= F * [[forall i : addr, imap i = option_map decode_inode (x0 i)]]  *
-    [[forall (i : addr) (inode : Inode),
-      imap i = Some inode -> compatible_inode imap i inode]]).
-      split; eauto.
-      pred_apply' H0; cancel.
-    }
-    split_ors; cleanup.
-    - left; exists x1; intuition cleanup.
-      destruct_lifts.
-      rewrite H5, H0; simpl; eauto.
-    pred_apply; cancel.
-    exists (upd x0 x1 (encode_inode (Build_Inode user []))).
-    pred_apply; cancel.
-    destruct (addr_dec x1 i); subst;
-    [ repeat rewrite upd_eq | repeat rewrite upd_ne]; simpl; eauto.
-    rewrite inode_encode_decode; eauto.
-
-    unfold compatible_inode in *;
-    destruct (addr_eq_dec x1 i); subst;
-    [ repeat rewrite upd_eq | repeat rewrite upd_ne]; simpl; eauto.
-    rewrite upd_eq in H2; eauto; cleanup.
-    simpl; intuition eauto.
-    constructor.
-    rewrite upd_ne in H3; eauto.
-    specialize H4 with (1:=H3); cleanup; eauto.
-
-    rewrite upd_ne in H2; eauto; cleanup.
-    specialize H4 with (1:= H2); cleanup.
-    intuition.
-     destruct (addr_eq_dec x1 j); subst;
-    [ repeat rewrite upd_eq | repeat rewrite upd_ne]; simpl; eauto.
-     rewrite upd_eq in H7; eauto; cleanup.
-     simpl.
-     rewrite app_nil_r.
-     specialize H4 with (2:= H2); cleanup; eauto.
-     rewrite upd_ne in H7; eauto.
-    
-  - right; intuition cleanup.
-    pred_apply; cancel.
-    exists x0.
-    pred_apply; cancel.
-
-  - simpl; intros; cleanup.
-   apply pimpl_exists_l_star_r in H0.
-   destruct H0.
-   exists x0; eauto.    
-Qed.
-
-
-Theorem free_ok:
-  forall inum s' t imap F,
-    strongest_postcondition (TransactionalDiskLang data_length) (free inum)
-                            (fun o s => (F * inode_rep imap)%predicate (mem_union (fst s) (snd s)) /\
-                            (forall tok, In tok o -> tok <> OpOracle (TransactionalDiskOperation data_length) [TxnFull])%list ) t s' ->
-    (t = Some tt /\ (F * inode_rep (delete imap inum))%predicate (mem_union (fst s') (snd s'))) \/
-    (t = None /\ (F * inode_rep imap)%predicate (mem_union (fst s') (snd s'))).
-Proof.
-    unfold inode_rep; intros; simpl in *; cleanup.
-  eapply sp_impl in H.
-  eapply (sp_exists_extract (disk value)) with (P:=fun inode_block_map o s =>  (F *
-   (block_allocator_rep inode_block_map *
-    [[forall i : addr, imap i = option_map decode_inode (inode_block_map i)]] *
-           [[forall (i : addr) (inode : Inode),
-             imap i = Some inode -> compatible_inode imap i inode]]))%predicate
-                                                                          (mem_union (fst s) (snd s)) /\
-                                               (forall tok, In tok o -> tok <> OpOracle (TransactionalDiskOperation data_length) [TxnFull])%list) in H.
-    cleanup.
-    eapply sp_impl in H.
-    apply free_ok in H.
-    2: {
-      intros; cleanup.
-      simpl; eauto.
-      instantiate (1:= x0).
-      instantiate (1:= F * [[forall i : addr, imap i = option_map decode_inode (x0 i)]] *
-           [[forall (i : addr) (inode : Inode),
-             imap i = Some inode -> compatible_inode imap i inode]]).
-      split; eauto.
-      pred_apply' H0; cancel.
-    }
-    
-    split_ors; cleanup.
-  - left; intuition cleanup.
-    pred_apply; cancel.
-    exists (delete x0 inum).
-    pred_apply; cancel.
-    unfold delete.
-    destruct (addr_dec i inum); eauto.
-
-    unfold delete, compatible_inode in *;
-    destruct (addr_dec i inum); subst;
-    [ repeat rewrite upd_eq | repeat rewrite upd_ne]; simpl; eauto.
-    cleanup.
-    
-    specialize H3 with (1:=H1); cleanup; eauto.
-    simpl; intuition eauto.
-     destruct (addr_dec j inum); subst;
-    [ repeat rewrite upd_eq | repeat rewrite upd_ne]; simpl; eauto; cleanup.
-    
-  - right; intuition cleanup.
-    pred_apply; cancel.
-    exists x0.
-    pred_apply; cancel.
-
-  - simpl; intros; cleanup.
-   apply pimpl_exists_l_star_r in H0.
-   destruct H0.
-   exists x0; eauto.   
-Qed.
-
-Theorem extend_ok:
-  forall inum block_num s' t imap F,
-    strongest_postcondition (TransactionalDiskLang data_length) (extend inum block_num)
-                            (fun o s => (F * inode_rep imap)%predicate (mem_union (fst s) (snd s)) /\ free_block_number imap block_num /\
-                            (forall tok, In tok o -> tok <> OpOracle (TransactionalDiskOperation data_length) [TxnFull])%list ) t s' ->
-    (exists inode, imap inum = Some inode /\ t = Some tt /\ (F * inode_rep (upd imap inum (Build_Inode inode.(owner) (inode.(block_numbers)++[block_num]))))%predicate (mem_union (fst s') (snd s'))) \/
-    (t = None /\ (F * inode_rep imap)%predicate (mem_union (fst s') (snd s'))).
-Proof.
-  unfold extend; intros; cleanup.
-  apply sp_bind in H.
-  simpl in *; cleanup.
-  
-  eapply sp_impl in H;
-  [> eapply get_inode_ok in H; eauto
-  |try solve [intros; cleanup; simpl; intuition eauto] ].
-  cleanup.
-
-  apply sp_bind in H0.
-  simpl in *; cleanup.
-  eapply sp_impl in H2;
-  [> eapply set_inode_ok in H2; eauto
-  |try solve [intros; cleanup; simpl; intuition eauto] ].  
-  split_ors; cleanup.
-  
-  + cleanup; left; eexists; intuition eauto.
-    cleanup; eauto.
-  + right; intuition eauto.
-  + simpl; intros.
-    eapply sp_impl in H3;
-    [> eapply get_inode_ok in H3; eauto
-    |].
-    instantiate (2:= F * [[forall tok, In tok o -> tok <> OpOracle (TransactionalDiskOperation data_length) [TxnFull]%list ]] *
-                     [[ free_block_number imap block_num ]] ) in H3.
-    cleanup; destruct_lift H4.
-    split; eauto.
-    
-    unfold inode_rep in *; destruct_lifts.
-    apply pimpl_exists_l_star_r in H4.
-    destruct H4.
-    destruct_lift H4.
-    split; unfold compatible_inode in *; simpl.
-    unfold free_block_number in *.
-    split.
-    apply NoDup_app_comm; simpl.
-    constructor; eauto.    
-    symmetry in H;
-    specialize H10 with (1:= H);
-    cleanup; eauto.
-    
-    intros.
-    apply NoDup_app_comm.
-    rewrite app_assoc.
-    apply NoDup_app_comm.
-    simpl in *.
-    constructor.
-    unfold not; intros.
-    apply in_app_or in H7; split_ors;    
-    try solve [eapply H8; [|eauto]; eauto].
-    edestruct H10; eauto.
-    
-    simpl; intros; eauto.
-
-    simpl; intros; cleanup.
-    pred_apply; cancel.
-    eapply H6; eauto.
-    
-  + simpl in *; cleanup.
-    eapply sp_impl in H0;
-    [> eapply get_inode_ok in H0; eauto
-    |try solve [intros; cleanup; simpl; intuition eauto] ].
-    cleanup.
-    right; intuition.
-Qed.
-
-
-Theorem change_owner_ok:
-  forall inum user s' t imap F,
-    strongest_postcondition (TransactionalDiskLang data_length) (change_owner inum user)
-                            (fun o s => (F * inode_rep imap)%predicate (mem_union (fst s) (snd s)) /\
-                            (forall tok, In tok o -> tok <> OpOracle (TransactionalDiskOperation data_length) [TxnFull])%list ) t s' ->
-    (exists inode, imap inum = Some inode /\ t = Some tt /\ (F * inode_rep (upd imap inum (Build_Inode user (inode.(block_numbers)))))%predicate (mem_union (fst s') (snd s'))) \/
-    (t = None /\ (F * inode_rep imap)%predicate (mem_union (fst s') (snd s'))).
-Proof.
-  unfold change_owner; intros; cleanup.
-  apply sp_bind in H.
-  simpl in *; cleanup.
-  
-  eapply sp_impl in H;
-  [> eapply get_inode_ok in H; eauto
-  |try solve [intros; cleanup; simpl; intuition eauto] ].
-  cleanup.
-
-  apply sp_bind in H0.
-  simpl in *; cleanup.
-  eapply sp_impl in H2;
-  [> eapply set_inode_ok in H2; eauto
-  |try solve [intros; cleanup; simpl; intuition eauto] ].  
-  split_ors; cleanup.
-  
-  + cleanup; left; eexists; intuition eauto.
-    cleanup; eauto.
-  + right; intuition eauto.
-  + simpl; intros.
-    eapply sp_impl in H3;
-    [> eapply get_inode_ok in H3; eauto
-    |].
-    instantiate (2:= F * [[forall tok, In tok o -> tok <> OpOracle (TransactionalDiskOperation data_length) [TxnFull]%list ]] *
-                [[forall (i : addr) (inode : Inode),
-             imap i = Some inode -> compatible_inode imap i inode]]) in H3.
-    cleanup; destruct_lift H4.
-    split; eauto.
-    symmetry in H; specialize H8 with (1:= H).
-    unfold compatible_inode in *; simpl; cleanup; eauto.
-
-    simpl; intros; eauto.
-
-    simpl; intros; cleanup.
-    pred_apply; cancel.
-    eapply H5; eauto.
-
-    unfold inode_rep in *; destruct_lifts.
-    apply pimpl_exists_l_star_r in H4.
-    destruct H4.
-    destruct_lift H4; eauto.
-    
-  + simpl in *; cleanup.
-    eapply sp_impl in H0;
-    [> eapply get_inode_ok in H0; eauto
-    |try solve [intros; cleanup; simpl; intuition eauto] ].
-    cleanup.
-    right; intuition.
-Qed.
-
-Theorem get_block_number_ok:
-  forall inum off s' t imap F,
-    strongest_postcondition (TransactionalDiskLang data_length) (get_block_number inum off)
-                            (fun o s => (F * inode_rep imap)%predicate (mem_union (fst s) (snd s))) t s' ->
-    (exists inode, imap inum = Some inode /\ t = nth_error inode.(block_numbers) off /\ (F * inode_rep imap)%predicate (mem_union (fst s') (snd s'))) \/
-    (t = None /\ imap inum = None /\ (F * inode_rep imap)%predicate (mem_union (fst s') (snd s'))).
-Proof.
-  unfold get_block_number; intros; cleanup.
-  apply sp_bind in H.
-  simpl in *; cleanup.
-    
-  eapply sp_impl in H;
-  [> eapply get_inode_ok in H; eauto
-  |try solve [intros; cleanup; simpl; intuition eauto] ].
-  cleanup.
-  
-  + simpl in *; cleanup; left; eexists; intuition eauto.
-    eapply get_inode_ok in H0; eauto.
-    cleanup; eauto.
-  + simpl in *; cleanup; right; intuition eauto.
-    eapply get_inode_ok in H0; eauto.
-    cleanup; eauto.
-Qed.
-
-
-Theorem get_block_numbers_ok:
-  forall inum s' t imap F,
-    strongest_postcondition (TransactionalDiskLang data_length) (get_block_numbers inum)
-                            (fun o s => (F * inode_rep imap)%predicate (mem_union (fst s) (snd s))) t s' ->
-    (exists inode, imap inum = Some inode /\ t = Some inode.(block_numbers) /\ (F * inode_rep imap)%predicate (mem_union (fst s') (snd s'))) \/
-    (t = None /\ imap inum = None /\ (F * inode_rep imap)%predicate (mem_union (fst s') (snd s'))).
-Proof.
-  unfold get_block_numbers; intros; cleanup.
-  apply sp_bind in H.
-  simpl in *; cleanup.
-    
-  eapply sp_impl in H;
-  [> eapply get_inode_ok in H; eauto
-  |try solve [intros; cleanup; simpl; intuition eauto] ].
-  cleanup.
-  
-  + simpl in *; cleanup; left; eexists; intuition eauto.
-    eapply get_inode_ok in H0; eauto.
-    cleanup; eauto.
-    
-  + simpl in *; cleanup; right; intuition eauto.
-    eapply get_inode_ok in H0; eauto.
-    cleanup; eauto.
-Qed.
-
-Theorem get_owner_ok:
-  forall inum s' t imap F,
-    strongest_postcondition (TransactionalDiskLang data_length) (get_owner inum)
-                            (fun o s => (F * inode_rep imap)%predicate (mem_union (fst s) (snd s))) t s' ->
-    (exists inode, imap inum = Some inode /\ t = Some inode.(owner) /\ (F * inode_rep imap)%predicate (mem_union (fst s') (snd s'))) \/
-    (t = None /\ imap inum = None /\ (F * inode_rep imap)%predicate (mem_union (fst s') (snd s'))).
-Proof.
-  unfold get_block_numbers; intros; cleanup.
-  apply sp_bind in H.
-  simpl in *; cleanup.
-    
-  eapply sp_impl in H;
-  [> eapply get_inode_ok in H; eauto
-  |try solve [intros; cleanup; simpl; intuition eauto] ].
-  cleanup.
-  
-  + simpl in *; cleanup; left; eexists; intuition eauto.
-    eapply get_inode_ok in H0; eauto.
-    cleanup; eauto.
-    
-  + simpl in *; cleanup; right; intuition eauto.
-    eapply get_inode_ok in H0; eauto.
-    cleanup; eauto.
-Qed.
-*)
-Global Opaque alloc free extend change_owner get_block_number get_block_numbers get_owner.
+Global Opaque alloc free extend change_owner get_block_number get_all_block_numbers get_owner.
 
